src/CPolIRs.v
@@ -21,6 +21,8 @@ Module CPolIRs <: POLIRS with Module Instr := CInstr.
    Module Loop := Loop CInstr.
    Parameter scop_scheduler: OpenScop -> result OpenScop.
    Parameter phase_scop_scheduler: OpenScop -> result (OpenScop * OpenScop).
+   Parameter identity_tiling_phase_scop_scheduler:
+     OpenScop -> result (OpenScop * OpenScop).
    Parameter phase_scop_scheduler_with_iss :
      OpenScop -> result (OpenScop * OpenScop).
    Parameter diamond_phase_scop_scheduler :
@@ -49,6 +51,8 @@ Module CPolIRs <: POLIRS with Module Instr := CInstr.
    Definition export_for_pluto_phase_pipeline := export_for_phase_scheduler.
    Definition to_phase_openscop := export_for_phase_scheduler.
    Definition run_pluto_phase_pipeline := phase_scop_scheduler.
+   Definition run_pluto_identity_tiling_pipeline :=
+     identity_tiling_phase_scop_scheduler.
    Definition run_pluto_phase_pipeline_with_iss :=
      phase_scop_scheduler_with_iss.
    Definition run_pluto_diamond_phase_pipeline :=
